Def n-dimentional smooth manifold M is a connected metric space with an open covering ${u_i}$

1 ) $\forall \alpha, \exists h_\alpha: U_\alpha \rightarrow B = \{x \in R^n: ||x|| < 1\}$

2 ) if $U_\alpha \cap U_\beta = \emptyset$ then $h_\alpha \circ h_\beta = h_\beta \circ h_\alpha$ is differentiable and $\forall x \in h_\beta ( U_\alpha \cap U_\beta )$ det $Dln(x) \neq 0$

Remark: such point of M has a neighborhood homeomorphic to B

Remark: Roughtly speaking, M is a smooth manifold if for every $x_n \in M$ , $\exists N = N(x_0)$ 

Ex: $S= {x \in R^2: x_1 + x_2^2 = 1}$ is a smooth manifold

Th: Stabe manifold theorem :

$$\dot{x} = f(x) \quad (1)$$

$$f: E \rightarrow R^n, E \in R^n \text{ an open subset}, o \in E, f(0)=0, f \in C^1(E)$$

$\Phi_t :  E \rightarrow E$ is the flow generated by $(1)$

o is a hyperbolic equilibrium point

A=Df(0) has K eignevalues with $Re \lambda < 0$
n.k eignevalues with $Re \lambda = 0$

$$ \dot{x} = Ax \quad (2)$$

Then E k dimentional smooth manifold S, tengent to stable subset $E^s$ of (2) at 0, forall t >= 0 $\Phi_t(t) \subset S$,


There exists n-k-dimentional smooth manifold U, tengent to unstable susbstace $E^s$ of (2) of 0, forall t >= 0 $\Phi_t(t) \subset U$

(could not get the end)

I) If A has k eigenvalues with RE(lambda) < 0, and n-k eigenvalues with RE(lambda) > 0, then $\exists C \neq 0$ such that

$$ B = C^{-1} A C = diag[P, Q] = \begin{pmatrix} P & 0 \\ 0 & Q \end{pmatrix}$$

where P is a k x k matrix with all eigenvalues < 0, and Q is a n-k x n-k matrix with all eigenvalues > 0

where eigenvalues $\lambda_1 \dots \lambda_k$ of P
have negative real parts, eigevalues $\lambda_{k+1} \dots \lambda_n$ of Q have positive real 

II) System (1) can be written in the form 

$$ \dot{x} = Ax + F(x),$$
where $ \forall r>0, \exists \delta > 0$ such that 

$$ ||F(x)|| \leq \delta \Rightarrow ||F(x) - F(y)|| \leq \epsilon||x-y||$$
Indeed, $A= Df(0), F(x)= f(x) - Ax \Rightarrow F(0) = 0, DF(0) = 0$

III) Letting $y = C^{-1}x$, in the system

$$ \dot{x} = Ax + F(x) \Rightarrow \dot{y} = C^{-1} \dot{x} = C^{-1} A C y + C^{-1} F(Cy)$$

$$ G(x) - G(y) || = || C^{-1} F(Cy) - C^{-1} F(Cx) || \leq ||C^{-1}|| ||F(Cy) - F(Cx)|| \\
\leq ||C^{-1}|| \epsilon ||x-y||$$

Therefore, instead (1) , we can consider 

$$ \dot{y} = By + G(y) \quad (3)$$

where $B = \begin{pmatrix} P & 0 \\ 0 & Q \end{pmatrix}$, $Re \lambda(P) < 0, Re \lambda(Q) > 0$,

$$ ||G(y_1) - G(y_2)|| \leq \epsilon ||y_1 - y_2||$$

In the proof , it will be shown that there exits a n-k $C^1$ function $ \Psi_j$ : 

$$y_j = \Psi_j(y_1 \dots, y_x), j=\bar{k+1, n}$$

define k-dimentional manifold $\bar{S}$ is y span. Then after linear transformation $x=Cy$ we obtain the required S in subspace

Sketch of the proof ;  Introcude U(t) = $\begin{pmatrix}
e^{pt} & 0 \\
0 & 0 \end{pmatrix}$

$V(t) = \begin{pmatrix}
0 & 0 \\
0 & e^{qt} \end{pmatrix}$

U(0) + V(0) = I

$$ \dot{U(t)} = BU, \dot{V(t)} = BV$$ and $e^{Bt} = U(t) + V(t)$$

$$u(t,a) = U(t)a + \int_0^t U(t-s)G(U(s)a)ds - \int_0^t V(t-s)G(u(s)a)ds \quad (4)$$

We can solve (4) with the succesive approximation method : 

$$ u^{j+1}(t,a) = U(t)a + \int_0^t U(t-s)G(u^{(j)}(s)a)ds - \int_0^t V(t-s)G(u^{(j)}(s)a)ds$$


It can be proved, u^(j) converges to u(t,a) uniformly on $(0, +\infty) \times \{ || a || < \frac{\delta}{2k}\}$

Let us consider $u = \begin{pmatrix} u_1 \\ \vdots \\ u_n \end{pmatrix}$

Let's look at (4) again : 

$$
u(t,a) = U(t)a + \int_0^t U(t-s)G(u(s)a)ds - \int_0^t V(t-s)G(u(s)a)ds
$$

$$
u_j(0,a)= - (\int_t^\infty V(-s)G(u(s, a_1 \dots, a_n))ds)_j
$$

$$
\Psi_j(a_1 \dots, a_k) = u_j( \infty, a_1 \dots, a_k)
$$
(to recheck )

We put $\bar{S} = \{ y \in R^n | y_j = \Psi_j(y_1 \dots, y_n), j=\bar{k+1, n}, \sqrt{\sum_{j=k+1}^n y_i^2 } < \frac{\delta}{2k} \}$

Then $S = C\bar{S}$

$$\forall y(0) + \tilde{S} \forall t \geq 0, y(t,y(0)) \in \tilde{S}$$

moreover, it can be proved that 

$$
\frac{\partial \Psi_j}{\partial y_i}(0) = 0
$$

Son the tangent subspace to (7) of 0 is given by

$$\{y\in R^n | y_{k+1} = y_{k+1} = ... = 0  \}$$

The existence of unstable manifoldes $ \tilde{U}$ can be proved after changing the variable "t" to "-t",

Then the stable manifold of $\dot{y} = By - G(y)$ will be the unstable manifold of $\tilde{U}$ of (3)

Corollary : Under the hypothses of the Stable Manifold Theorem, $ \forall \epsilon > 0, \exists \delta > 0$ such that

$$ \forall x_0 \in S \cap N_\delta(\bar{0}), || \Phi_t(x_0) || \leq \epsilon e^{-\alpha t}, \forall t \geq 0$$

$$ \forall x_0 \in S \cap N_\delta(\bar{0}), || \Phi_t(x_0) || \leq \epsilon e^{-\beta t}, \forall t \leq 0$$

Exemple : 

$$\begin{cases}
\dot{x_1} = -x_1 - x_2^2 \\
\dot{x_2} = x_1^2 - x_2
\end{cases}$$

$$
A = Df(\bar{0}) \begin{pmatrix}
-1 & 0 \\
0 & 1
\end{pmatrix}
$$

The eigenvalues are $ \lambda_1 = -1, \lambda_2 = 1$

Let's find u^{(1)}(t,a) and u^{(2)}(t,a) : and use $u^{(2)}$ to approximate stable manifold

$$
u(t,a) = \begin{pmatrix}
e^{-t} & 0 \\	
0 & 0
\end{pmatrix}a + \int_0^t \begin{pmatrix}
e^{-(t-s)} & 0 \\
0 & 0
\end{pmatrix} \begin{pmatrix} - u_1(s,a)^2 \\ u_2(s,a)^2
\end{pmatrix}ds - \int_t^\infty \begin{pmatrix}
0 & 0 \\ 0 & e^{(t-s)}
\end{pmatrix} \begin{pmatrix} - u_1(s,a)^2 \\ u_2(s,a)^2
\end{pmatrix}ds
$$

Succesive approximation method :

$$
u^{(0)}(t,0) = 0 \\
u^{(1)}(t,a) = \begin{pmatrix}
a_1 e^{-t} \\ 0
\end{pmatrix} \\
u^{(2)}(t,a) = \begin{pmatrix}
a_1 e^{-t} \\ - \frac{1}{3} e_1^2 e^{-2t}
\end{pmatrix}
$$

We take "approximately"" $u^{(2)} \approx u(t,a)$





  






